Get ml_optimiseTheory and ml_pmatchTheory to build

translator/ml_pmatchScript.sml
@@ -11,154 +11,45 @@ val write_def = ml_progTheory.write_def;
 
 val EvalPatRel_def = Define`
   EvalPatRel env a p pat ⇔
-    ∀x av. a x av ⇒
-      evaluate_match F env empty_state av
+    ∀x av. a x av ⇒ ∀refs.
+      evaluate_match F env (empty_state with refs := refs) av
         [(p,Con NONE [])] ARB
-        (empty_state,
+        (empty_state with refs := refs,
          if ∃vars. pat vars = x
          then Rval(Conv NONE []) else Rerr(Rraise ARB))`
 
-val Pmatch_def = tDefine"Pmatch"`
-  (Pmatch env [] [] = SOME env) ∧
-  (Pmatch env (p1::p2::ps) (v1::v2::vs) =
-     case Pmatch env [p1] [v1] of | NONE => NONE
-     | SOME env' => Pmatch env' (p2::ps) (v2::vs)) ∧
-  (Pmatch env [Pvar x] [v] = SOME (write x v env)) ∧
-  (Pmatch env [Plit l] [Litv l'] =
-     if l = l' then SOME env else NONE) ∧
-  (Pmatch env [Pcon (SOME n) ps] [Conv (SOME (n',t')) vs] =
-     case lookup_alist_mod_env n env.c of
-      | NONE => NONE
-     | SOME (l,t) =>
-       if same_tid t t' ∧ LENGTH ps = l ∧
-          same_ctor (id_to_n n, t) (n',t')
-       then Pmatch env ps vs
-       else NONE) ∧
-  (Pmatch env [Pcon NONE ps] [Conv NONE vs] =
-     if LENGTH ps = LENGTH vs then
-       Pmatch env ps vs
-     else NONE) ∧
-  (Pmatch env _ _ = NONE)`
-  (WF_REL_TAC`measure (pat1_size o FST o SND)`)
-
-val Pmatch_ind = theorem"Pmatch_ind"
-
 val EvalPatBind_def = Define`
   EvalPatBind env a p pat vars env2 ⇔
-    ∃x av.
+    ∃x av refs env'.
       a x av ∧
-      (Pmatch env [p] [av] = SOME env2) ∧
+      (pmatch env.c refs p av env.v = Match env') ∧
+      (env2 = env with v := env') ∧
       (pat vars = x)`
-
-val Pmatch_cons = store_thm("Pmatch_cons",
-  ``∀ps vs.
-      Pmatch env (p::ps) (v::vs) =
-      case Pmatch env [p] [v] of | NONE => NONE
-      | SOME env' => Pmatch env' ps vs``,
-  Induct >> Cases_on`vs` >> simp[Pmatch_def] >>
-  BasicProvers.CASE_TAC >>
-  Cases_on`ps`>>simp[Pmatch_def])
-
-val Pmatch_SOME_const = store_thm("Pmatch_SOME_const",
-  ``∀env ps vs env'.
-      Pmatch env ps vs = SOME env' ⇒
-      env'.m = env.m ∧
-      env'.c = env.c``,
-  ho_match_mp_tac Pmatch_ind >> simp[Pmatch_def] >>
-  rw[] >> BasicProvers.EVERY_CASE_TAC >> fs[] >>
-  fs[write_def])
-
-val pmatch_imp_Pmatch = prove(
-  ``(∀envC s p v env aenv.
-      s = empty_store ⇒
-      envC = aenv.c ∧ env = aenv.v ⇒
-      case pmatch envC s p v aenv.v of
-      | Match env' =>
-        Pmatch aenv [p] [v] = SOME (aenv with v := env')
-      | _ => Pmatch aenv [p] [v] = NONE) ∧
-    (∀envC s ps vs env aenv.
-      s = empty_store ⇒
-      envC = aenv.c ∧ env = aenv.v ⇒
-      case pmatch_list envC s ps vs aenv.v of
-      | Match env' =>
-        Pmatch aenv ps vs = SOME (aenv with v := env')
-      | _ => Pmatch aenv ps vs = NONE)``,
-  ho_match_mp_tac pmatch_ind >>
-  rw[pmatch_def,Pmatch_def,write_def]
-  >> TRY (rw[environment_component_equality]>>NO_TAC)
-  >- (
-    BasicProvers.CASE_TAC >>
-    BasicProvers.CASE_TAC >>
-    BasicProvers.CASE_TAC >> fs[] >>
-    BasicProvers.CASE_TAC >> fs[] )
-  >- (
-    BasicProvers.CASE_TAC >>
-    BasicProvers.CASE_TAC >>
-    BasicProvers.CASE_TAC >>
-    fs[store_lookup_def] >>
-    fs[empty_store_def])
-  >- (
-    first_x_assum(qspec_then`aenv`mp_tac)>>simp[]>>
-    BasicProvers.CASE_TAC >> fs[] >>
-    simp[Once Pmatch_cons] >>
-    BasicProvers.CASE_TAC >> fs[] >>
-    simp[Once Pmatch_cons] >> rw[Pmatch_def] >>
-    first_x_assum(qspec_then`aenv with v := a`mp_tac)>>simp[]>>
-    BasicProvers.CASE_TAC >> simp[Once Pmatch_cons])
-  >- (
-    Cases_on`v110`>>simp[Pmatch_def]))
-  |> SIMP_RULE std_ss []
-  |> curry save_thm "pmatch_imp_Pmatch"
-
-val Pmatch_imp_pmatch = store_thm("Pmatch_imp_pmatch",
-  ``∀env ps vs env'.
-      (Pmatch env ps vs = SOME env' ⇒
-       pmatch_list env.c empty_store ps vs env.v =
-         Match env'.v) ∧
-      (Pmatch env ps vs = NONE ⇒
-       ∀env2.
-       pmatch_list env.c empty_store ps vs env.v ≠
-         Match env2)``,
-  ho_match_mp_tac Pmatch_ind >>
-  simp[Pmatch_def,pmatch_def] >> rw[] >>
-  fs[write_def] >>
-  BasicProvers.CASE_TAC >> fs[] >>
-  BasicProvers.EVERY_CASE_TAC >> rfs[] >> rw[] >>
-  imp_res_tac Pmatch_SOME_const >>
-  fs[write_def] >>
-  rfs[] >>
-  Cases_on`v20`>>fs[pmatch_def] >>
-  BasicProvers.EVERY_CASE_TAC >> fs[store_lookup_def,empty_store_def])
 
 val pmatch_PMATCH_ROW_COND_No_match = store_thm("pmatch_PMATCH_ROW_COND_No_match",
   ``EvalPatRel env a p pat ∧
     (∀vars. ¬PMATCH_ROW_COND pat (K T) xv vars) ∧
     a xv res ⇒
-    Pmatch env [p] [res] = NONE``,
+    pmatch env.c refs p res env.v = No_match``,
   fs [PMATCH_ROW_COND_def] >>
   rw[EvalPatRel_def] >>
   first_x_assum(fn th => first_x_assum(strip_assume_tac o MATCH_MP th)) >>
-  qspecl_then[`p`,`res`,`env`]strip_assume_tac(CONJUNCT1 pmatch_imp_Pmatch)
-  \\ Cases_on `Pmatch env [p] [res]` \\ fs []
-  \\ Cases_on `pmatch env.c empty_store p res env.v` \\ fs []
-  \\ SRW_TAC [] [] \\ rw[Once evaluate_cases,PMATCH_ROW_COND_def] \\ fs []
-  \\ REPEAT STRIP_TAC \\ SRW_TAC [] [] \\ rfs[]
-  \\ REPEAT (POP_ASSUM MP_TAC)
-  \\ NTAC 4 (fs[Once evaluate_cases,PMATCH_ROW_COND_def,empty_state_def]));
+  first_x_assum(qspec_then`refs`mp_tac) >>
+  ntac 4 (simp[Once evaluate_cases]) >>
+  rw[pmatch_def]);
 
 val pmatch_PMATCH_ROW_COND_Match = store_thm("pmatch_PMATCH_ROW_COND_Match",
   ``EvalPatRel env a p pat ∧
     PMATCH_ROW_COND pat (K T) xv vars ∧
     a xv res
-    ⇒ ∃env2. Pmatch env [p] [res] = SOME env2``,
+    ⇒ ∃env2. pmatch env.c refs p res env.v = Match env2``,
   rw[EvalPatRel_def,PMATCH_ROW_COND_def] >>
   first_x_assum(fn th => first_x_assum(strip_assume_tac o MATCH_MP th)) >>
-  qspecl_then[`p`,`res`,`env`]strip_assume_tac(CONJUNCT1 pmatch_imp_Pmatch) >>
-  fs[Once evaluate_cases] >> rfs[] >>
-  BasicProvers.EVERY_CASE_TAC >> fs[] >>
-  fs[Once evaluate_cases] >>
-  fs[empty_state_def] >>
-  PROVE_TAC[]);
+  first_x_assum(qspec_then`refs`mp_tac) >>
+  ntac 4 (fs[Once evaluate_cases]) >>
+  strip_tac \\ every_case_tac \\ fs[] \\
+  fs[pmatch_def] \\ fs[Once evaluate_cases] \\
+  metis_tac[]);
 
 val Eval_PMATCH_NIL = store_thm("Eval_PMATCH_NIL",
   ``!b x xv a.
@@ -166,8 +57,6 @@ val Eval_PMATCH_NIL = store_thm("Eval_PMATCH_NIL",
       CONTAINER F ==>
       Eval env (Mat x []) (b (PMATCH xv []))``,
   rw[CONTAINER_def]);
-
-val empty_state_refs = EVAL``empty_state.refs = empty_store`` |> EQT_ELIM
 
 val Eval_PMATCH = store_thm("Eval_PMATCH",
   ``!b a x xv.
@@ -184,49 +73,42 @@ val Eval_PMATCH = store_thm("Eval_PMATCH",
       Eval env (Mat x ((p,e)::ys)) (b (PMATCH xv ((PMATCH_ROW pat (K T) res)::yrs)))``,
   rw[Eval_def] >>
   rw[Once evaluate_cases,PULL_EXISTS] >> fs[] >>
-  first_assum(match_exists_tac o concl) >> simp[] >>
+  first_x_assum(qspec_then`refs`strip_assume_tac) >>
+  asm_exists_tac \\ fs[] \\
   rw[Once evaluate_cases,PULL_EXISTS] >>
   Cases_on`∃vars. PMATCH_ROW_COND pat (K T) xv vars` >> fs[] >- (
     imp_res_tac pmatch_PMATCH_ROW_COND_Match >>
-    ntac 3 (pop_assum kall_tac) >>
+    pop_assum kall_tac >>
+    first_x_assum(qspec_then`refs++refs'`strip_assume_tac) \\ fs[] \\
+    qpat_x_assum`p1 xv ⇒ $! _`kall_tac >>
     fs[EvalPatRel_def] >>
-    first_x_assum(qspec_then`vars`mp_tac)>>simp[] >>
-    qpat_x_assum`p1 xv ⇒ X`kall_tac >>
-    fs[EvalPatBind_def,PMATCH_ROW_COND_def,PULL_EXISTS] >>
     first_x_assum(qspec_then`vars`mp_tac)>>simp[] >> strip_tac >>
     first_x_assum(fn th => first_assum(strip_assume_tac o MATCH_MP th)) >>
-    srw_tac[DNF_ss][] >> disj1_tac >>
-    imp_res_tac Pmatch_imp_pmatch >>
-    imp_res_tac Pmatch_SOME_const >>
-    fs[pmatch_def] >>
-    qpat_x_assum`X = Match Y` mp_tac >> BasicProvers.CASE_TAC >>
-    fs[GSYM AND_IMP_INTRO] >>
-    first_x_assum(fn th => first_assum(strip_assume_tac o MATCH_MP th)) >>
-    rfs[] >>
-    `(∃vars'. pat vars' = pat vars) = T` by metis_tac[] >>
-    fs[] >> rfs[] >>
-    simp[PMATCH_def,PMATCH_ROW_def,PMATCH_ROW_COND_def] >>
-    `(some x. pat x = pat vars) = SOME vars` by (
+    first_x_assum(qspec_then`refs++refs'`mp_tac) >>
+    ntac 4 (simp[Once evaluate_cases]) \\ rw[] \\
+    fs[PMATCH_ROW_COND_def] \\
+    `EvalPatBind env a p pat vars (env with v := env2)`
+    by (
+      simp[EvalPatBind_def,environment_component_equality] \\
+      metis_tac[] ) \\
+    first_x_assum drule \\ simp[]
+    \\ disch_then(qspec_then`refs++refs'`strip_assume_tac)
+    \\ full_simp_tac std_ss [GSYM APPEND_ASSOC]
+    \\ asm_exists_tac \\ fs[]
+    \\ simp[PMATCH_def,PMATCH_ROW_def,PMATCH_ROW_COND_def] >>
+    `(some x. pat x = pat vars') = SOME vars` by (
       simp[optionTheory.some_def] >>
       METIS_TAC[] ) >>
-    simp[] >> fs[] >> rw[] >>
-    fs[pmatch_def,empty_state_refs] >>
-    rw[] >>
-    `env2 = env with v := env2.v` by rw[environment_component_equality] >>
-    METIS_TAC[]) >>
-  qpat_x_assum`evaluate F X Y (Mat A B) R`mp_tac >>
+    simp[]) >>
+  first_x_assum(qspec_then`refs`strip_assume_tac) \\
+  qpat_x_assum`evaluate F _ _ (Mat _ _) _`mp_tac >>
   simp[Once evaluate_cases] >> strip_tac >>
   imp_res_tac (CONJUNCT1 big_exp_determ) >> fs[] >> rw[] >>
   srw_tac[DNF_ss][] >> disj2_tac >>
   simp[PMATCH_def,PMATCH_ROW_def] >>
   imp_res_tac pmatch_PMATCH_ROW_COND_No_match >>
-  imp_res_tac Pmatch_imp_pmatch >>
-  fs[pmatch_def] >>
-  pop_assum mp_tac >> BasicProvers.CASE_TAC >- (
-    fs[empty_state_refs] >> METIS_TAC[] ) >>
-  fs[EvalPatRel_def] >>
-  first_x_assum(fn th => first_x_assum(mp_tac o MATCH_MP th)) >>
-  simp[Once evaluate_cases,empty_state_refs] >> rw[]);
+  first_x_assum(qspec_then`refs++refs'`strip_assume_tac) >> fs[] >>
+  asm_exists_tac \\ fs[]);
 
 val PMATCH_option_case_rwt = store_thm("PMATCH_option_case_rwt",
   ``((case x of NONE => NONE
